reification WIP

src/Experiments/SpecificCurve25519.v
@@ -1,13 +1,283 @@
+Require Import Crypto.Util.GlobalSettings.
 Require Import Crypto.Util.Notations Coq.ZArith.BinInt.
 Require Import Crypto.Specific.GF25519.
 Require Import Crypto.CompleteEdwardsCurve.ExtendedCoordinates.
+Require Import Crypto.Tactics.VerdiTactics.
+
+Inductive type := TZ | Prod : type -> type -> type.
+
+Section expr.
+  Context {var : type -> Type}.
+  Inductive expr : type -> Type :=
+  | Const : Z -> expr TZ
+  | Var : forall {t}, var t -> expr t
+  | Binop : (Z->Z->Z) -> expr TZ -> expr TZ -> expr TZ
+  | Let : forall {tx}, expr tx -> forall {tC}, (var tx -> expr tC) -> expr tC
+  | Pair : forall {t1}, expr t1 -> forall {t2}, expr t2 -> expr (Prod t1 t2)
+  | MatchPair : forall {t1 t2}, expr (Prod t1 t2) -> forall {tC}, (var t1 -> var t2 -> expr tC) -> expr tC
+  .
+End expr.
+Arguments expr _ _ : clear implicits.
+Definition Expr t := forall var, expr var t.
+
+Fixpoint tinterp (t:type) :=
+  match t with
+  | TZ => Z
+  | Prod a b => prod (tinterp a) (tinterp b)
+  end.
+
+Fixpoint interp {t} (e:expr tinterp t) : tinterp t :=
+  match e in expr _ t return tinterp t with
+  | Const n => n
+  | Var _ n => n
+  | Binop op e1 e2 => op (interp e1) (interp e2)
+  | Let _ ex _ eC => interp (eC (interp ex))
+  | Pair _ e1 _ e2 => (interp e1, interp e2)
+  | MatchPair _ _ ep _ eC => let (v1, v2) := interp ep in interp (eC v1 v2)
+  end.
+
+Example example_expr : interp (Let (Const 7) (fun a => Let (Let (Binop Z.add (Var a) (Var a)) (fun b => Pair (Var b) (Var b))) (fun p => MatchPair (Var p) (fun x y => Binop Z.add (Var x) (Var y))) )) = 28%Z. reflexivity. Qed.
+
+Section unmatch_pair.
+  Context {var : type -> Type}.
+  Definition CoqPairIfPair {t1 t2} (ep : expr var (Prod t1 t2)) : option (expr var t1 * expr var t2)
+   := match ep in expr _ t return option (match t with
+                                          | Prod t1 t2 => (expr var t1 * expr var t2)
+                                          | _ => False
+                                          end) with
+      | Pair _ e1 _ e2 => Some (e1, e2)
+      | _ => None
+      end.
+
+  Fixpoint unmatch_pair {t} (e:expr var t) : expr var t :=
+    match e in expr _ t return expr var t with
+    | MatchPair _ _ ep _ eC
+      => match CoqPairIfPair (unmatch_pair ep) with
+         | Some (e1, e2) => Let e1 (fun v1 => (Let e2 (fun v2 => unmatch_pair (eC v1 v2))))
+         | None => MatchPair (unmatch_pair ep) (fun x y => unmatch_pair (eC x y))
+         end
+    | Const n => Const n
+    | Var _ n => Var n
+    | Binop op e1 e2 => Binop op (unmatch_pair e1) (unmatch_pair e2)
+    | Let _ ex _ eC => Let (unmatch_pair ex) (fun x => unmatch_pair (eC x))
+    | Pair _ e1 _ e2 => Pair (unmatch_pair e1) (unmatch_pair e2)
+    end.
+End unmatch_pair.
+
+Ltac simpl_lem_then_rewrite lem :=
+  let t := type of lem in
+  let t' := (eval simpl in t) in
+  let lem' :=  constr:(lem:t') in
+  rewrite lem'.
+
+Lemma CoqPairIfPair_Some_helper {var} {t} (ep:expr var t) :
+  match t return expr var t -> Prop with
+  | Prod _ _ => fun ep => forall e1 e2, CoqPairIfPair ep = Some (e1, e2) <-> ep = Pair e1 e2
+  | _ => fun _ => True
+  end ep.
+Proof.
+  unfold CoqPairIfPair; destruct ep; try break_match;
+    repeat (intuition congruence || match goal with [H:_ |- _] => apply (f_equal CoqPairIfPair) in H end).
+Qed.
+
+Lemma CoqPairIfPair_Some {var} {t1 t2} (ep:expr var (Prod t1 t2)) e1 e2 :
+    CoqPairIfPair ep = Some (e1, e2) <-> ep = Pair e1 e2.
+Proof.
+  simpl_lem_then_rewrite (CoqPairIfPair_Some_helper ep); reflexivity.
+Qed.
+
+Lemma unmatch_pair_correct : forall {t} (e:expr tinterp t), interp (unmatch_pair e) = interp e.
+  induction e; simpl;
+    try destruct (interp e) eqn:Heqe;
+    repeat break_match; simpl;
+    try find_apply_lem_hyp @CoqPairIfPair_Some;
+    repeat match goal with
+           | _ => solve [intuition]
+           | _ => progress simpl @interp in *
+           | [H: _ |- _ ] => rewrite H
+           | [H: _, H': _ |- _ ] => rewrite H in H'
+           | [H: (_, _) = (_, _) |- _ ] => inversion H; subst
+           end.
+Qed.
+Section reassoc_let.
+  Context {var : type -> Type}.
+
+  Definition matchLetLetInIn {t} (e:expr var t) :
+    option (sigT (fun tx:type => (expr var tx * (var tx -> expr var t))%type)) :=
+    match e with Let _ ex _ eC => Some (existT _ _ (ex, eC)) | _ => None end.
+
+  Fixpoint reassoc_let {t} (e:expr var t) {struct e} : expr var t :=
+    match e in expr _ t return expr var t with
+    | Let _ ex _ eC =>
+      match matchLetLetInIn ex with
+      | Some (existT tx' (ex', eC')) =>
+        Let ex' (fun v' => Let (eC' v') (fun v => reassoc_let (eC v)))
+      | None => Let (reassoc_let ex) (fun v => reassoc_let (eC v))
+      end
+    | Const n => Const n
+    | Var _ n => Var n
+    | Binop op e1 e2 => Binop op (reassoc_let e1) (reassoc_let e2)
+    | Pair _ e1 _ e2 => Pair (reassoc_let e1) (reassoc_let e2)
+    | MatchPair _ _ ep _ eC => MatchPair (reassoc_let ep) (fun x y => reassoc_let (eC x y))
+    end.
+End reassoc_let.
+
+Lemma matchLetLetInIn_Some {var} {t} (e:expr var t) {tx} ex eC :
+  matchLetLetInIn e = Some (existT _ tx (ex, eC)) <-> e = Let ex eC.
+Proof.
+  destruct e; simpl; intros; try intuition congruence.
+  split; intros; injection H; clear H; intros; subst.
+  admit.
+  admit.
+Admitted.
+
+Lemma reassoc_let_correct : forall {t} (e:expr tinterp t), interp (reassoc_let e) = interp e.
+  induction e;
+    repeat match goal with
+           | [H: _ |- _ ] => simpl_lem_then_rewrite H
+           | [H: _ |- _ ] => rewrite matchLetLetInIn_Some in H
+           | _ => break_match
+           | _ => progress simpl
+           | _ => progress subst
+           | _ => solve [intuition congruence]
+           end.
+Qed.
+
+
+
 Local Infix "<<" := Z.shiftr.
 Local Infix "&" := Z.land.
-
 Section Curve25519.
-  Context {twice_d : fe25519}.
-
-  Definition ge25519_add :=
+  Definition ge25519_add' (twice_d : fe25519) :=
     Eval cbv beta delta [Extended.add_coordinates fe25519 add mul sub ModularBaseSystemOpt.Let_In] in
       @Extended.add_coordinates fe25519 add sub mul twice_d.
+
+  Definition ge25519_add_sig (twice_d : fe25519) : forall P1 P2, { r | r = ge25519_add' twice_d P1 P2 }.
+    intros.
+    hnf in twice_d.
+    repeat match goal with p:prod _ _ |- _ => destruct p end.
+    eexists.
+    etransitivity.
+    Focus 2. {
+      cbv beta delta [ge25519_add'].
+      Set Printing All.
+
+Ltac reify_type t :=
+  lazymatch t with
+  | BinInt.Z => constr:(TZ)
+  | prod ?l ?r =>
+    let l := reify_type l in
+    let r := reify_type r in
+    constr:(Prod l r)
+  end.
+
+Ltac type_of x := match type of x with ?t => constr:(t) end.
+Ltac reify_type_of x :=
+  let t := type_of x in
+  reify_type t.
+Ltac rhs_of_goal := match goal with |- ?R ?LHS ?RHS => constr:(RHS) end.
+
+      let rhs := rhs_of_goal in
+      let t := reify_type_of rhs in
+      idtac t.
+
+Goal (0 = let x := 0 in x+x)%Z.
+
+Class reify {varT} (var:varT) {eT} (e:eT) {T:Type} := Build_reify : T.
+Definition reify_var_for_is {T} (x:T) t (e:tinterp t) := False.
+
+Ltac reify var e :=
+  lazymatch e with
+  | let x := ?ex in @?eC x =>
+    let ex := reify var ex in
+    let eC := reify var eC in
+    constr:(Let(var:=var) ex eC)
+  | ?op ?a ?b =>
+    let a := reify var a in
+    let b := reify var b in
+    constr:(Binop(var:=var) op a b)
+  | (fun x : ?T => @?C x) =>
+    let t := reify_type T in
+    lazymatch constr:(fun (x : T) (v : var t) (_:reify_var_for_is x t v) =>
+                        (_ : reify var ltac:(let Cx := eval cbv beta in (C x) in exact Cx)))
+    with fun _ v _ => @?C v => C end
+  | ?x =>
+    match goal with
+    | _:reify_var_for_is x ?t ?v |- _ => constr:(@Var var t v)
+    | _ => constr:(Const(var:=var) x)
+    end
+  end.
+Hint Extern 0 (reify ?var ?e) => (let e := reify var e in eexact e) : typeclass_instances.
+
+      let A := constr:(fun x:Z => (_:reify tinterp (Z.add 2 1))) in
+      idtac A.
+
+      Goal forall (x : Z) (v : tinterp TZ) (_:reify_var_for_is x TZ v), reify(T:=Z) tinterp ((fun x => x+x) x)%Z.
+        intros.
+        let A := reify tinterp (x + x)%Z in
+        idtac A.
+      Abort.
+
+      let A := reify tinterp (fun x => Z.add x x) in
+      idtac A.
+
+      let A := reify tinterp constr:(let x := Z0 in Z.add x x) in
+      idtac A.
+
+      let rhs := rhs_of_goal in
+      let rhs := reify tinterp rhs in
+      idtac rhs.
+
+
+| (fun x : ?T => @?f x)
+  => let T' := reify_TypeCode T in
+     let res := match constr:(Set) with
+                | _ => constr:(fun (x : T) (v : var T') (_:reify_as x 
+                               => let vx : reif_Term_of var x := (@RVar var T' v) in
+                                  (_ : reif_Term_of var (f x)))
+                | _ => cidtac_error "Unable to reify function" f
+                end in
+     let res := (eval cbv beta iota zeta in res) in
+     let res := match res with
+                | (fun _ => ?f) => f
+                | _ => cidtac_error "Unable to remove first argument to" f
+                end in
+     match constr:(Set) with
+     | _ => constr:(@RLambda var T' _ res)
+     | _ => cidtac_error "Type error" res
+     end
+
+
+
+                                              
+  | context G[match ?y with pair a b => @?f a b end]
+    => lazymatch eval hnf in y with
+    | pair _ _
+      => let G' := context G [Let_In (optfst y) (fun a => Let_In (optsnd y) (fun b => f a b))] in
+         from_let_in_to_Let_In_and_remove_pairs fuel' G'
+    | _
+      => let dummy := match y with
+                      | prod_rect _ _ ?y' => constr:(_ : is_local_context_var y')
+                      | _ => constr:(_ : is_local_context_var y)
+                      | _ => constr:(_ : cidtac "Warning: Term does not reduce to a pair:" y "")
+                      end in
+         let T := match type of f with _ -> _ -> ?T => T end in
+         let G' := context G [prod_rect (fun _ => T) f y] in
+         from_let_in_to_Let_In_and_remove_pairs fuel' G'
+    end
+  | ?f ?x
+    => let f' := from_let_in_to_Let_In_and_remove_pairs fuel' f in
+       let x' := from_let_in_to_Let_In_and_remove_pairs fuel' x in
+       constr:(f' x')
+  | fun x : ?T => @?f x
+    => let ret := constr:(fun x : T => (_ : from_let_in_to_Let_In_and_remove_pairs fuel' (f x))) in
+       let ret := (eval cbv beta delta [from_let_in_to_Let_In_and_remove_pairs] in ret) in
+       ret
+  | ?term'
+    => term'
+  end.
+
+      
+        
+
 End Curve25519.
